trying to prove vm = eval

Instr.v
@@ -113,15 +113,57 @@ Admitted.
 Definition parallel_att_vm_thread (li:list Instr) (e:Evidence) : COP Evidence.
 Admitted.
 
+Definition vm_prim_thread (i:Instr) (p:Plc) (e:Evidence) : COP Evidence.
+Admitted.
+
+Definition parallel_eval_cop_thread (t:Term) (p:Plc) (e:Evidence) : COP Evidence.
+Admitted.
+
 Definition splitEv (sp:SP) (e:Evidence) : Evidence :=
   match sp with
   | ALL => e
   | NONE => mt
   end.
 
+Definition eval_asp_cop (a:ASP) (p:Plc) (e:Evidence) : COP Evidence :=
+  match a with
+  | CPY => ret e
+  | KIM i q args =>
+    bs <- invokeKIM i q args ;;
+       ret (kk i args q p bs e)
+  | USM i args =>
+    bs <- invokeUSM i args ;;
+       ret (uu i args p bs e)
+  | SIG =>
+    bs <- signEv e ;;
+       ret (gg p e bs)
+  | HSH =>
+    bs <- hashEv e ;;
+       ret (hh p bs)
+  end.
 
-Fixpoint vm_prim (e:Evidence) (instr:Instr) : COP Evidence :=
-  p <- asks me ;;
+Fixpoint eval_cop t p e :=
+  match t with
+  | asp a => eval_asp_cop a p e
+  | att q t1 => eval_cop t1 q e
+  | lseq t1 t2 =>
+    e1 <- eval_cop t1 p e ;;
+       eval_cop t2 p e1
+  | bseq (sp1,sp2) t1 t2 =>
+    let e1 := splitEv sp1 e in
+    let e2 := splitEv sp2 e in
+    e1' <- eval_cop t1 p e1 ;;
+        e2' <- eval_cop t2 p e2 ;;
+        ret (ss e1' e2')
+  | bpar (sp1,sp2) t1 t2 =>
+    let e1 := splitEv sp1 e in
+    let e2 := splitEv sp2 e in
+    e1' <- parallel_eval_cop_thread t1 p e1 ;;
+        e2' <- parallel_eval_cop_thread t2 p e2 ;;
+        ret (pp e1' e2')
+  end.
+
+Definition vm_prim (p:Plc) (e:Evidence) (instr:Instr) : COP Evidence :=
     match instr with
     | copy => ret e
     | kmeas i q args =>
@@ -155,14 +197,14 @@ Fixpoint vm_prim (e:Evidence) (instr:Instr) : COP Evidence :=
     | besl ev' =>
       match e with
       | sp e1 e2 =>
-        e1' <- vm_prim e1 ev' ;;
+        e1' <- vm_prim_thread ev' p e1 ;; (*vm_prim p e1 ev' ;; *)
             ret (sp e1' e2)
       | _ => ret mt (* TODO: throw "bad stack" error? *)
       end
     | besr ev' =>
       match e with
       | sp e1 e2 =>
-        e2' <- vm_prim e2 ev' ;;
+        e2' <- vm_prim_thread ev' p e2 ;;(*vm_prim p e2 ev' ;; *)
             ret (sp e1 e2')
       | _ => ret mt (* TODO: throw "bad stack" error? *)
       end
@@ -176,5 +218,49 @@ Fixpoint vm_prim (e:Evidence) (instr:Instr) : COP Evidence :=
       end
     end.
 
-Fixpoint att_vm (is:list Instr) (e:Evidence) : COP Evidence :=
-  foldM_COP vm_prim e is.
+Check foldM_COP.
+
+Fixpoint att_vm (is:list Instr) (p:Plc) (e:Evidence) : COP Evidence :=
+  foldM_COP (vm_prim p) e is.
+
+(*
+Lemma asdf : forall e,
+IdentityMonad.unIdent
+  (ReaderMonad.runReaderT (vm_prim e copy) empty_cop_env) = e.
+Proof.
+  intros. simpl.
+Admitted. *)
+  
+Theorem eval_vm : forall (t:Term) (p:Plc) (e:Evidence) env,
+    runCOP (eval_cop t p e) env = runCOP (att_vm (instr_compiler t p) p e) env.
+Proof.
+  intros.
+  generalize dependent p; intros.
+  induction t.
+  + 
+    destruct a; try (cbv; reflexivity).
+  + admit.
+  + unfold eval_cop
+    
+    
+  + destruct env. simpl.
+    
+  - simpl. destruct env.
+
+    simpl. unfold empty_cop_env.
+    assert (p = 0). admit. congruence
+    unfold instr_compiler. unfold asp_instr.
+    unfold att_vm. unfold foldM_COP. unfold eval_cop. unfold eval_asp_cop
+
+
+  simpl.
+  unfold runCOP at 1. simpl. unfold runCOP at 1.
+  simpl.
+  unfold runCOP. simpl. unfold ReaderMonad.runReaderT.
+  unfold vm_prim
+  destruct empty_cop_env. simpl. unfold vm_prim.
+  destruct runReaderT.
+  destruct env
+  simpl. unfold vm_prim
+  
+  
