MonadCOP.v
@@ -2,6 +2,9 @@ Require Import Term.
 Require Import Coq.ZArith.ZArith_base Coq.Strings.String Coq.Strings.Ascii.
 Require Import ExtLib.Data.Monads.StateMonad ExtLib.Data.Monads.ReaderMonad ExtLib.Structures.Monads ExtLib.Data.Monads.IdentityMonad.
 
+Require Import List.
+Import ListNotations.
+
 Record Cop_Env : Type := mkCop_Env
                            { nameServer : NS ;
                              me : Plc}.
@@ -9,3 +12,8 @@ Record Cop_Env : Type := mkCop_Env
 (* ident is the identity monad, acting as a place-holder for the base monad.
    TODO:  eventually we need this to be IO (or something that models IO) *)
 Definition COP := readerT Cop_Env (ident).
+
+Definition runCOP {A:Type} (k:(COP A)) (env:Cop_Env) : A (* (A * AM_St)*) :=
+  unIdent (runReaderT k env).
+
+Definition empty_cop_env := (mkCop_Env [] 0).
